Cleaned up insertion sort

examples/algorithms/insertionsort.fst
@@ -17,42 +17,52 @@
 
 module InsertionSort
 open Prims.PURE
+open List
 
 (* Check that a list is sorted *)
 val sorted: list int -> Tot bool
 let rec sorted l = match l with
-    | [] -> true
-    | [x] -> true
-    | x::y::xs -> x <= y && sorted (y::xs)
+    | [] | [_] -> true
+    | x::y::xs -> (x <= y) && (sorted (y::xs))
 
-val test_sorted: x:int -> l:list int -> Lemma ((sorted (x::l) /\ is_Cons l) ==> x <= Cons.hd l)
+val test_sorted: x:int -> l:list int ->
+      Lemma ((sorted (x::l) /\ is_Cons l) ==> x <= Cons.hd l)
 let test_sorted x l = ()
 
 val test_sorted2: unit -> Tot (m:list int{sorted m})
 let test_sorted2 () = Nil
 
 (* Fact about sorted *)
-val mem: 'a -> list 'a -> Tot bool
-let rec mem a l = match l with
-  | [] -> false
-  | hd::tl -> hd=a || mem a tl
-
-val sorted_smaller: x:int -> y:int -> l:list int ->
-                    Lemma (sorted (x::l) /\ mem y l ==> x <= y)
+val sorted_smaller: x:int
+                ->  y:int
+                ->  l:list int
+                ->  Lemma (requires (sorted (x::l) /\ mem y l))
+                          (ensures (x <= y))
+                          [SMTPat (sorted (x::l)); SMTPat (mem y l)]
 let rec sorted_smaller x y l = match l with
     | [] -> ()
     | z::zs -> if z=y then () else sorted_smaller x y zs
 
-val insert : i:int -> l:list int{sorted l} -> Tot (m:list int{sorted m /\ (forall x. mem x m <==> x==i \/ mem x l)})
+(* Explicitly calling lemma *)
+val insert : i:int -> l:list int{sorted l} ->
+      Tot (m:list int{sorted m /\ (forall x. mem x m <==> x==i \/ mem x l)})
 let rec insert i l = match l with
   | [] -> [i]
   | hd::tl ->
-     if i <= hd
-     then i::l
+     if i <= hd then i::l
      else let i_tl = insert i tl in 
           let (z::_) = i_tl in
-          sorted_smaller hd z tl; (* need to call the lemma explicitly, currently *)
+          if mem z tl then sorted_smaller hd z tl;
           hd::i_tl
+
+(* Solver implicitly uses the lemma: sorted_smaller hd (Cons.hd i_tl) tl *)
+val insert_implicit : i:int -> l:list int{sorted l} ->
+      Tot (m:list int{sorted m /\ (forall x. mem x m <==> x==i \/ mem x l)})
+let rec insert_implicit i l = match l with
+  | [] -> [i]
+  | hd::tl ->
+     if i <= hd then i::l
+     else hd::(insert_implicit i tl)
 
 (* Insertion sort *)
 val sort : l:list int -> Tot (m:list int{sorted m /\ (forall x. mem x l == mem x m)})
